```lisp
;; f(n)=n if n<3
;; f(n)=f(n−1) + 2f(n−2) + 3f(n−3) if n≥3n

#lang racket

(define (f n)
  (if (< n 3) 
      n 
      (+ (f (- n 1))
         (* 2 (f (- n 2)))
         (* 3 (f (- n 3))))))

(f 1)
(f 2)
(f 3)
(f 4)
(f 5)
(f 6)

;; f(0) = 0
;; f(1) = 1
;; f(2) = 2
;; f(3) = f(2) + 2 * f(1) + 3 * f(0)
;; f(4) = f(3) + 2 * f(2) + 3 * f(1)

(define (ff n)
   (define (f-iter a b c count)
     (if (= count 0)
         a
         (f-iter b c (+ c (* 2 b) (* 3 a)) (- count 1))))
   (f-iter 0 1 2 n)
)

(ff 1)
(ff 2)
(ff 3)
(ff 4)
(ff 5)
(ff 6)

```

> PARTIALLY CORRECT. Needed to reflect on solution for iterative approach

